src/Narcissus/Formats/PermutationOpt.v
@@ -384,7 +384,7 @@ Section Resilience.
   Qed.
 End Resilience.
 
-Section Permutation.
+Section PermutationToList.
 
   (* Since identity is a permutation, composing with permutations
   refines to no composition*)
@@ -419,7 +419,10 @@ Section Permutation.
 
   (* Turns any element into a list, given projections for all it's
   components*)
-  Fixpoint to_list {n:nat} {S:Type} {types:Vector.t Type n}:
+  (* Old version
+     The new version is more compositional
+   *)
+  Fixpoint to_list' {n:nat} {S:Type} {types:Vector.t Type n}:
     forall projections: ilist (B:= fun T => S -> T) types, 
       S -> list (SumType types):=
     match types as typs return
@@ -430,9 +433,37 @@ Section Permutation.
         let typs:= Vector.cons Type a n' typs' in
         fun projs S =>
           (inj_SumType typs Fin.F1 (prim_fst projs S))
-            :: map (lift_SumType a) (to_list (prim_snd projs) S)
+            :: map (lift_SumType a) (to_list' (prim_snd projs) S)
     end.
 
+  
+
+  
+  (* Like a monadic operation
+     `??` in haskell
+   *)
+  Definition iapp {n:nat} {S:Type} {types:Vector.t Type n}
+    (fM: ilist (B:= fun T:Type => S -> T) types) (s:S)
+    : ilist (B:= id) types:=
+    @imap Type (fun T:Type => S -> T) id (fun _ f => f s) _ _ fM.
+        
+  Fixpoint ito_list {n:nat} {types:Vector.t Type n}:
+    ilist (B:=id) types -> list (SumType types):=
+    match types as typs return
+          ilist (B:=id) typs ->
+          list (SumType typs) with
+    | Vector.nil => constant Datatypes.nil
+    | @Vector.cons _ a n' typs' =>
+        let typs:= Vector.cons Type a n' typs' in
+        fun ils =>
+          (inj_SumType typs Fin.F1 (prim_fst ils))
+            :: map (lift_SumType a) (ito_list (prim_snd ils))
+    end.
+
+  Definition to_list {n:nat} {S:Type} {types:Vector.t Type n}
+    (projs: ilist (B:= fun T:Type => S -> T) types):= fun s => ito_list (iapp projs s).
+  
+  
   (* Format for lists of SumTypes. *)
   Definition SumType_list_Format
              (m : nat) (types : Vector.t Type m)
@@ -504,9 +535,975 @@ Section Permutation.
         eapply IndexedSumType_resilience; auto.
       + apply IndexedSumType_Encoder_Correct; assumption.
   Qed.
+
+
+  
+  (** *The Decoder*)
+Lemma EquivFormat_compose_projection {T S S' S''}
+              (format_S'' : FormatM S'' T)
+              (f : S -> S')
+              (r : S' -> S'' -> Prop)
+          : EquivFormat (Projection_Format (Compose_Format format_S'' r) f)
+                        (Compose_Format format_S'' (fun a b => r (f a) b)).
+        Proof.
+          unfold EquivFormat, refineEquiv, Projection_Format, Compose_Format, compose, Bind2; split;
+            intros ? ?.
+          - rewrite unfold_computes in *.
+            destruct_ex; split_and; eexists.
+            rewrite unfold_computes;  eauto.
+          - rewrite unfold_computes in *.
+            destruct_ex; split_and.
+            rewrite unfold_computes in H0.
+            destruct_ex; split_and.
+            eexists; intuition eauto.
+            subst; eauto.
+        Qed.
+
+        Ltac normalize_step BitStringT ::=
+          (first
+             [ match goal with
+               | |- EquivFormat ?z ?x => is_evar z; apply EquivFormat_reflexive
+               end; idtac "1"
+             | eapply EquivFormat_trans; [ apply sequence_assoc |  ]
+               ; idtac "3"
+             | eapply EquivFormat_trans;
+               [ apply sequence_mempty with (monoid := BitStringT) |  ]
+               ; idtac "5"
+             | eapply EquivFormat_ComposeIf; intros
+               ; idtac "6"
+             | eapply EquivFormat_trans;
+               [ apply EquivFormat_If_Then_Else with (monoid := BitStringT) |  ]
+               ; idtac "8"
+             | apply EquivFormat_If_Then_Else_Proper
+               ; idtac "9"
+             | eapply EquivFormat_UnderSequence';
+               [ repeat
+                   (eapply EquivFormat_trans;
+                    [ first [eapply EquivFormat_compose_map; idtac "10.0" |
+                              eapply EquivFormat_compose_projection; idtac "10.1" ] |  ] );
+                 apply EquivFormat_reflexive
+               |  ] ; idtac "10"
+             | eapply EquivFormat_Projection_Format_Empty_Format';
+               [ repeat eapply EquivFormat_compose_map;
+                 apply EquivFormat_reflexive ] ; idtac "11"
+             | unfold EquivFormat; intros; reflexivity ]); 
+          intros.
+
+Lemma to_list_length:
+  forall S n (types: Vector.t Type n) (s:S) (projs: ilist types) ,
+    (| to_list projs s |) = n.
+Proof.
+  intros ??; induction types.
+  - intros. reflexivity.
+  - intros. simpl.
+    f_equal; rewrite map_length.
+    eapply IHtypes.
+Qed.
+
+
+    Definition permutation_decoder
+      {m S}
+      {types : Vector.t Type m}
+      (fin_decoder : ByteString ->
+                CacheDecode ->
+                option (Fin.t m * ByteString * CacheDecode))
+      (decoders : ilist
+                    (B:= fun T : Type => @DecodeM (T * ByteString) ByteString
+                                        EmptyStore.test_cache) types)
+      (decode2 : list (SumType types) ->
+                 DecodeM (S * ByteString) ByteString)
+       :=
+      (sequence_Decode
+       (decode_list (decoder_IndexedSumType fin_decoder decoders)
+          m) decode2).
+
+
+    (*
+DecodeM = 
+fun (S T : Type) (store : Cache) => T -> CacheDecode -> option (S * CacheDecode)
+     *)
+      
+(* Easier to proof version.
+  The better version to automate below
+ *)
+Lemma Permutation_decoder': 
+  forall (S: Type) m (types: Vector.t Type m)
+    (projs: ilist (B:= fun T => S -> T) types) (cache_inv: CacheDecode -> Prop)
+    (cache_invariants: Vector.t ((_ -> Prop) -> Prop) m) fin_cache_inv
+    (fin_format : FormatM (Fin.t m) ByteString)
+    fin_decoder view_fin
+    (fin_correct: cache_inv_Property cache_inv fin_cache_inv ->
+                        CorrectDecoder ByteStringQueueMonoid view_fin 
+                          view_fin eq fin_format fin_decoder cache_inv fin_format)
+    (formats : ilist types)
+    (source_pred : S -> Prop),
+    cache_inv_Property cache_inv
+      (fun P : CacheDecode -> Prop =>
+         fin_cache_inv P /\
+           IterateBoundedIndex.Iterate_Ensemble_BoundedIndex
+             (fun idx : Fin.t m => Vector.nth cache_invariants idx P)) ->
+    forall (invariants: ilist (B:= fun T : Type => T -> Prop) types)
+          (decoders: ilist (B:=fun T => DecodeM (T * ByteString) ByteString) types)
+          (formatrs_decoders_correct :
+            IterateBoundedIndex.Iterate_Ensemble_BoundedIndex
+              (fun idx =>
+                 cache_inv_Property cache_inv (Vector.nth cache_invariants idx)
+                 -> CorrectDecoder
+                     ByteStringQueueMonoid
+                     (ith invariants idx)
+                     (ith invariants idx)
+                     eq
+                     (ith formats idx)
+                     (ith decoders idx)
+                     cache_inv
+                     (ith formats idx)))
+        (Hinvariants_ok: forall (s : S) (v : list (SumType types)),
+            source_pred s ->
+            Permutation (to_list projs s) v ->
+            forall x : SumType types,
+              In x (to_list projs s) ->
+              view_fin (SumType_index types x) /\
+                ith invariants (SumType_index types x) (SumType_proj types x))
+        format2 (decode2: list (SumType types) -> DecodeM (S * ByteString) ByteString)
+        (P_inv2:(CacheDecode -> Prop) -> Prop)
+        (Hcache_inv2: cache_inv_Property cache_inv
+           (fun P : CacheDecode -> Prop =>
+              (fin_cache_inv P /\
+                 IterateBoundedIndex.Iterate_Ensemble_BoundedIndex'
+                   (fun idx : Fin.t m => Vector.nth cache_invariants idx P)) /\
+                P_inv2 P))
+        (Decoder2_Correct: forall v1 : list (SumType types),
+                     cache_inv_Property cache_inv P_inv2 ->
+                     (| v1 |) = m /\
+                     (forall x : SumType types,
+                      In x v1 ->
+                      view_fin (SumType_index types x) /\
+                      ith invariants (SumType_index types x) (SumType_proj types x)) ->
+                     CorrectDecoder ByteStringQueueMonoid
+                       (fun s : S => source_pred s /\ Permutation (to_list projs s) v1)
+                       (fun s : S => source_pred s /\ Permutation (to_list projs s) v1) eq format2
+                       (decode2 v1) cache_inv format2)
+        ,
+          CorrectDecoder ByteStringQueueMonoid
+                  source_pred source_pred
+                           eq 
+                           (@permutation_Format
+                              S m types projs fin_format formats
+                              ++ format2
+                           )
+                           (permutation_decoder fin_decoder decoders decode2)
+                           cache_inv
+                           (@permutation_Format
+                              S m types projs fin_format formats
+                              ++ format2
+           ).
+Proof.
+  (* Real goal*)
+  unfold permutation_Format, permutation_list_Format, SumType_list_Format.
+  normalize_format. (*10.1, 10, 10*)
+  eapply sequence_Compose_format_decode_correct; cycle 1.
+  intros.
+  (* eapply strengthen_view_pred_Proper; unfold flip, pointwise_relation, impl; cycle 1. *)
+  (* eapply weaken_view_predicate_Proper; unfold flip, pointwise_relation, impl. cycle 1. *)
+  (* eapply weaken_source_pred_Proper; unfold flip, pointwise_relation, impl; simpl; cycle 1. *)
+     (* weaken_view_predicate_Proper
+      strengthen_view_pred_Proper *)
     
-        
-End Permutation.
+    (*1*) intros; apply FixList_decode_correct.
+  eapply IndexedSumType_Decoder_Correct; eassumption; eassumption; eassumption.
+  - simpl. intros s v Hsource Hperm.
+    split.
+    + eapply Permutation_length in Hperm.
+      rewrite <- Hperm. 
+      eapply to_list_length. 
+    + intros ??;
+        eapply Hinvariants_ok; eauto. 
+      eapply Permutation_in; [symmetry|];  eassumption.
+  - simpl.
+    eapply Decoder2_Correct.
+  - simpl. simpl.
+    assumption.
+Qed.
+
+(* Some lemmas to modifiy themake the statment amenable to automation*)
+
+Lemma SumType_index_lift:
+  forall n (types : Vector.t Type n) (h: Type) (y : SumType types),
+    (SumType_index (Vector.cons Type h n types) (lift_SumType h y)) =
+      Fin.FS (SumType_index types y).
+Proof.
+  destruct types.
+  - intros; elim y.
+  - reflexivity.
+Qed.
+
+Lemma SumType_proj_lift:
+  forall n (types : Vector.t Type n) (h: Type) (y : SumType types),
+    let types':= (Vector.cons Type h n types) in
+    SumType_proj types y ~= SumType_proj types' (lift_SumType h y)
+.
+Proof.
+  destruct types.
+  - intros. elim y.
+  - reflexivity.
+Qed.
+
+Lemma SumType_proj_in_list:
+  forall { S : Type} {m : nat} (types : Vector.t Type m) (projs : ilist(B:= (fun T : Type => S -> T)) types) s x, 
+    In x (to_list projs s) ->
+    ith projs (SumType_index types x) s = SumType_proj types x.
+Proof.
+  induction types.
+  - intros. elim H.
+  - intros. destruct projs as [pi0 projs].
+    unfold to_list, iapp in H.
+    simpl imap in H.
+    Lemma ito_list_cons:
+      forall {n} {T:Type} {types : Vector.t Type n} (x0: T) (ils: ilist(B:=id) types),  
+        let typs := Vector.cons Type T n types in
+        ito_list (icons x0 ils) =
+          inj_SumType typs Fin.F1 x0 :: map (lift_SumType T) (@ito_list n types ils).
+    Proof. reflexivity. Qed.
+
+    rewrite ito_list_cons in H. 
+    destruct H; cycle 1.
+    + eapply in_map_iff in H.
+      destruct H as (y &Heqxy & H).
+      eapply IHtypes in H.
+      etransitivity; [rewrite <- Heqxy| reflexivity].
+      assert (LHS_lemma:
+               forall n (types : Vector.t Type n) (h: Type) (y : SumType types) S (s:S) ,
+                 let types':= (Vector.cons Type h n types) in
+                 forall (projs : ilist (B:=fun T : Type => S -> T) types'),
+                   ith projs (SumType_index types' (lift_SumType h y)) s ~=
+                     ith projs (Fin.FS (SumType_index types y)) s).
+      {
+        clear; intros.
+        subst types'.
+        erewrite SumType_index_lift.
+        econstructor.
+      }
+      eapply JMeq_eq.
+      etransitivity.
+      eapply LHS_lemma.
+      simpl.
+      rewrite H.
+
+      eapply SumType_proj_lift.
+
+    + clear IHtypes.
+      rewrite <- H.
+      destruct types; reflexivity.
+Qed.
+
+
+Lemma In_implies_Iterated:
+  forall n S types (s:S) projs (pred: Fin.t n -> Prop),
+    IterateBoundedIndex.Iterate_Ensemble_BoundedIndex pred ->
+    (forall (x : SumType types),
+        In x (@to_list n S types projs s) ->
+        pred (SumType_index types x)).
+Proof.
+  intros.
+  eapply IterateBoundedIndex.Iterate_Ensemble_BoundedIndex_equiv in H.
+  instantiate (1:= SumType_index types x) in H.
+  eauto.
+Qed.
+
+(* Version of the lemma written for automation. See each hypothesis for details about why it changed*)
+Lemma Permutation_decoder: 
+  forall (S: Type) m (types: Vector.t Type m)
+    (projs: ilist (B:= fun T => S -> T) types) (cache_inv: CacheDecode -> Prop)
+    (cache_invariants: Vector.t ((_ -> Prop) -> Prop) m) fin_cache_inv
+    (fin_format : FormatM (Fin.t m) ByteString)
+    fin_decoder view_fin
+    (fin_correct: cache_inv_Property cache_inv fin_cache_inv ->
+                        CorrectDecoder ByteStringQueueMonoid view_fin 
+                          view_fin eq fin_format fin_decoder cache_inv fin_format)
+    (formats : ilist types)
+    (source_pred : S -> Prop),
+    cache_inv_Property cache_inv
+      (fun P : CacheDecode -> Prop =>
+         fin_cache_inv P /\
+           IterateBoundedIndex.Iterate_Ensemble_BoundedIndex
+             (fun idx : Fin.t m => Vector.nth cache_invariants idx P)) ->
+    forall (invariants: ilist (B:= fun T : Type => T -> Prop) types)
+          (decoders: ilist (B:=fun T => DecodeM (T * ByteString) ByteString) types)
+          (formatrs_decoders_correct :
+            IterateBoundedIndex.Iterate_Ensemble_BoundedIndex
+              (fun idx =>
+                 cache_inv_Property cache_inv (Vector.nth cache_invariants idx)
+                 -> CorrectDecoder
+                     ByteStringQueueMonoid
+                     (ith invariants idx)
+                     (ith invariants idx)
+                     eq
+                     (ith formats idx)
+                     (ith decoders idx)
+                     cache_inv
+                     (ith formats idx)))
+        (* Change the hypothesis to use
+        `Iterate_Ensemble_BoundedIndex`, so it can easily be unfolded
+        into the list of subproofs. *)
+        (Hinvariants_ok: forall (s : S) (v : list (SumType types)),
+            source_pred s ->
+            Permutation (to_list projs s) v ->
+            IterateBoundedIndex.Iterate_Ensemble_BoundedIndex
+              (fun idx =>
+                 view_fin idx /\
+                   ith invariants idx (ith projs idx s)
+              ))
+        format2 (decode2: list (SumType types) -> DecodeM (S * ByteString) ByteString)
+        (P_inv2:(CacheDecode -> Prop) -> Prop)
+        (Hcache_inv2: cache_inv_Property cache_inv
+           (fun P : CacheDecode -> Prop =>
+              (fin_cache_inv P /\
+                 IterateBoundedIndex.Iterate_Ensemble_BoundedIndex'
+                   (fun idx : Fin.t m => Vector.nth cache_invariants idx P)) /\
+                P_inv2 P))
+        (Decoder2_Correct: forall v1 : list (SumType types),
+                     cache_inv_Property cache_inv P_inv2 ->
+                     (| v1 |) = m /\
+                     (forall x : SumType types,
+                      In x v1 ->
+                      view_fin (SumType_index types x) /\
+                      ith invariants (SumType_index types x) (SumType_proj types x)) ->
+                     CorrectDecoder ByteStringQueueMonoid
+                       (fun s : S => source_pred s /\ Permutation (to_list projs s) v1)
+                       (fun s : S => source_pred s /\ Permutation (to_list projs s) v1) eq format2
+                       (decode2 v1) cache_inv format2)
+        ,
+          CorrectDecoder ByteStringQueueMonoid
+                  source_pred source_pred
+                           eq 
+                           (@permutation_Format
+                              S m types projs fin_format formats
+                              ++ format2
+                           )
+                           (permutation_decoder fin_decoder decoders decode2)
+                           cache_inv
+                           (@permutation_Format
+                              S m types projs fin_format formats
+                              ++ format2
+                           ).
+Proof.
+  intros.
+  eapply Permutation_decoder'; try eassumption.
+  - (* Turn a quantification of every item in a list with `In`, to an
+    iteration ver all the elements with
+    `Iterate_Ensemble_BoundedIndex`*)
+
+      clear - Hinvariants_ok.
+      intros.
+      remember (fun idx => view_fin (idx) /\ ith invariants (idx) (ith projs idx s)) as pred.
+      replace (SumType_proj types x) with (ith projs (SumType_index types x) s); cycle 1.
+      { revert H1.
+        eapply SumType_proj_in_list.
+      }
+      cut ((fun y => view_fin y /\ ith invariants y (ith projs y s)) (SumType_index types x)); [simpl; auto|].
+      eapply In_implies_Iterated; eauto.
+Qed.
+
+
+
+  
+End PermutationToList.
+
+Section Permutation.
+(* We simplify the decoder to finish with a ilist, so we can ensure it
+can be built back into an S*)
+
+   
+  
+  (** *The decoder*)
+  Definition BindSum {A B err} (a_sum: A + err) (k: A -> B + err): B + err:=
+    match a_sum with
+    | inl a =>
+        match k a with
+        | inl b => inl b
+        | inr e => inr e
+        end
+    | inr e => inr e
+    end.
+  Definition BindOpt2 {B1 B2 C} := fun a b => @BindOpt (B1*B2) C a (fun x => b (fst x) (snd x)).  
+  Delimit Scope option_scope with option.
+  Notation "x <- y ; z" := (BindOpt y%option (fun x => z%option))
+                           (at level 81, right associativity,
+                             format "'[v' x  <-  y ; '/' z ']'") : option_scope.
+  Notation "`( a , b ) <- c ; k" :=
+    (BindOpt2 c%option (fun a b => k%option))
+      (at level 81, right associativity,
+        format "'[v' `( a ,  b )  <-  c ; '/' k ']'") : option_scope.
+  Declare Scope sum_scope.
+  Notation "x <- y ; z" := (BindSum y (fun x => z))
+                           (at level 81, right associativity,
+                            format "'[v' x  <-  y ; '/' z ']'") : sum_scope.
+  Delimit Scope sum_scope with sum.
+  Open Scope option_scope.
+
+
+  (*| If the element has the first type, it returns the element.
+      Otherwise, it returns the element in a lowered SumType.
+      Specifically, if removes the first type from the Sum.
+   *)
+  Fixpoint extract_lowest
+    {m: nat} {T: Type} {types : Vector.t Type m}:
+    let types' := Vector.cons Type T _ types in
+    SumType types' -> (SumType types + T):=    
+  (* Proof. *)
+  (*   simpl; intros. *)
+  (*   destruct types. *)
+  (*   - left; exact X. *)
+  (*   - destruct X. *)
+  (*     + left. exact t. *)
+  (*     + right; eauto. *)
+  (* Defined. *)
+    match
+      types as t in (Vector.t _ n)
+      return (SumType (Vector.cons Type T n t) -> SumType t + T)
+    with
+    | @Vector.nil _ => fun a => inr a
+    | @Vector.cons _ h n types0 =>
+        fun a => match a with
+          | inl a => inr a
+          | inr y => inl y
+          end
+    end.
+
+  Fixpoint mapOpt {A B} (f: A -> option B) (ls: list A): option (list B):=
+    match ls with
+    | [] => Some []
+    | x::ls' =>
+        y <- f x;
+        ls_b' <- mapOpt f ls';
+        Some (y :: ls_b')
+  end.
+  Fixpoint mapSum {A B T} (f: A -> B + T) (ls: list A): (list B + T):=
+    match ls with
+    | [] => inl []
+    | x::ls' =>
+        (y <- f x;
+        ls_b' <- mapSum f ls';
+        inl (y :: ls_b'))%sum
+    end.
+
+  (* If any element has the first type, it returns the element.
+     Otherwise, it removes that type from the list.
+   *)
+  Fixpoint lower_SumTypes
+    {m: nat} {T: Type} {types : Vector.t Type m}:
+    let types' := Vector.cons Type T _ types in
+    list (SumType types') -> (list (SumType types) + T):=
+    mapSum extract_lowest.
+  
+    Fixpoint remove_fst_type
+    {m: nat} {T: Type} {types : Vector.t Type m}
+    (ls: list (SumType (Vector.cons Type T _ types))):
+      option (T * list (SumType types)):=
+      match ls with
+      | [] => None
+      | x :: ls0 =>
+          match extract_lowest x with
+          | inl xx => x_ls' <- remove_fst_type ls0;
+                     Some (fst x_ls', xx :: (snd x_ls'))
+          | inr t => match lower_SumTypes ls0 with
+                    | inl ls' => Some (t, ls')
+                    | inr _ => (* In this case there where two elems of the same type*)
+                        None
+                    end
+           end
+  end.
+  
+  Fixpoint sortType {m} {types : Vector.t Type m}
+    (ls: list (SumType types)): option (ilist (B:=id) types):=
+    match
+    types as t in (Vector.t _ n)
+    return (list (SumType t) -> option (ilist t))
+    with
+    | @Vector.nil _ => constant Some ()
+    | @Vector.cons _ h n types0 =>
+        fun ls0 : list (SumType (Vector.cons Type h n types0)) =>
+          match remove_fst_type ls0 with
+          | Some (t, ls1) =>
+              match sortType ls1 with
+              | Some i => Some {| prim_fst := t; prim_snd := i |}
+              | None => None
+              end
+          | None => None
+          end
+    end ls.
+  
+  Definition permutation_decoder_ilist
+    {m S}
+    {types : Vector.t Type m}
+    (fin_decoder : ByteString ->
+                   CacheDecode ->
+                   option (Fin.t m * ByteString * CacheDecode))
+    (decoders : ilist
+                  (B:= fun T : Type => @DecodeM (T * ByteString) ByteString
+                                      EmptyStore.test_cache) types)
+    (decode2 : ilist (B:=id) types ->
+               DecodeM (S * ByteString) ByteString): DecodeM (S * ByteString) ByteString:=
+    permutation_decoder fin_decoder decoders  (fun x => Ifopt sortType x as ils Then decode2 ils Else (fun  _ _ => None)).  
+
+
+  (** Correctness lemma *)
+
+        Ltac normalize_step BitStringT ::=
+          (first
+             [ match goal with
+               | |- EquivFormat ?z ?x => is_evar z; apply EquivFormat_reflexive
+               end; idtac "1"
+             | eapply EquivFormat_trans; [ apply sequence_assoc |  ]
+               ; idtac "3"
+             | eapply EquivFormat_trans;
+               [ apply sequence_mempty with (monoid := BitStringT) |  ]
+               ; idtac "5"
+             | eapply EquivFormat_ComposeIf; intros
+               ; idtac "6"
+             | eapply EquivFormat_trans;
+               [ apply EquivFormat_If_Then_Else with (monoid := BitStringT) |  ]
+               ; idtac "8"
+             | apply EquivFormat_If_Then_Else_Proper
+               ; idtac "9"
+             | eapply EquivFormat_UnderSequence';
+               [ repeat
+                   (eapply EquivFormat_trans;
+                    [ first [eapply EquivFormat_compose_map; idtac "10.0" |
+                              eapply EquivFormat_compose_projection; idtac "10.1" ] |  ] );
+                 apply EquivFormat_reflexive
+               |  ] ; idtac "10"
+             | eapply EquivFormat_Projection_Format_Empty_Format';
+               [ repeat eapply EquivFormat_compose_map;
+                 apply EquivFormat_reflexive ] ; idtac "11"
+             | unfold EquivFormat; intros; reflexivity ]); 
+          intros.
+
+Lemma Permutation_decoder_ilist_Correct: 
+  forall (S: Type) m (types: Vector.t Type m)
+    (projs: ilist (B:= fun T => S -> T) types) (cache_inv: CacheDecode -> Prop)
+    (cache_invariants: Vector.t ((_ -> Prop) -> Prop) m) fin_cache_inv
+    (fin_format : FormatM (Fin.t m) ByteString)
+    fin_decoder view_fin
+    (fin_correct: cache_inv_Property cache_inv fin_cache_inv ->
+                        CorrectDecoder ByteStringQueueMonoid view_fin 
+                          view_fin eq fin_format fin_decoder cache_inv fin_format)
+    (formats : ilist types)
+    (source_pred : S -> Prop),
+    cache_inv_Property cache_inv
+      (fun P : CacheDecode -> Prop =>
+         fin_cache_inv P /\
+           IterateBoundedIndex.Iterate_Ensemble_BoundedIndex
+             (fun idx : Fin.t m => Vector.nth cache_invariants idx P)) ->
+    forall (invariants: ilist (B:= fun T : Type => T -> Prop) types)
+          (decoders: ilist (B:=fun T => DecodeM (T * ByteString) ByteString) types)
+          (formatrs_decoders_correct :
+            IterateBoundedIndex.Iterate_Ensemble_BoundedIndex
+              (fun idx =>
+                 cache_inv_Property cache_inv (Vector.nth cache_invariants idx)
+                 -> CorrectDecoder
+                     ByteStringQueueMonoid
+                     (ith invariants idx)
+                     (ith invariants idx)
+                     eq
+                     (ith formats idx)
+                     (ith decoders idx)
+                     cache_inv
+                     (ith formats idx)))
+        (Hinvariants_ok: forall (s : S) (v : list (SumType types)),
+            source_pred s ->
+            Permutation (to_list projs s) v ->
+            forall x : SumType types,
+              In x (to_list projs s) ->
+              view_fin (SumType_index types x) /\
+                ith invariants (SumType_index types x) (SumType_proj types x))
+        format2 (decode2: ilist types -> DecodeM (S * ByteString) ByteString)
+        (P_inv2:(CacheDecode -> Prop) -> Prop)
+        (Hcache_inv2: cache_inv_Property cache_inv
+           (fun P : CacheDecode -> Prop =>
+              (fin_cache_inv P /\
+                 IterateBoundedIndex.Iterate_Ensemble_BoundedIndex'
+                   (fun idx : Fin.t m => Vector.nth cache_invariants idx P)) /\
+                P_inv2 P))
+        ,
+          CorrectDecoder ByteStringQueueMonoid
+                  source_pred source_pred
+                           eq 
+                           (@permutation_Format
+                              S m types projs fin_format formats
+                              ++ format2
+                           )
+                           (permutation_decoder_ilist fin_decoder decoders decode2)
+                           cache_inv
+                           (@permutation_Format
+                              S m types projs fin_format formats
+                              ++ format2
+           ).
+Proof.
+  
+  (* Real goal*)
+  unfold permutation_Format, permutation_list_Format, SumType_list_Format.
+  normalize_format. (*10.1, 10, 10*)
+  eapply sequence_Compose_format_decode_correct; cycle 1.
+  intros.
+  (* eapply strengthen_view_pred_Proper; unfold flip, pointwise_relation, impl; cycle 1. *)
+  (* eapply weaken_view_predicate_Proper; unfold flip, pointwise_relation, impl. cycle 1. *)
+  (* eapply weaken_source_pred_Proper; unfold flip, pointwise_relation, impl; simpl; cycle 1. *)
+     (* weaken_view_predicate_Proper
+      strengthen_view_pred_Proper *)
+    
+  - (*1*) intros; apply FixList_decode_correct.
+    eapply IndexedSumType_Decoder_Correct; eassumption; eassumption; eassumption.
+  - simpl. intros s v Hsource Hperm.
+    split.
+    + eapply Permutation_length in Hperm.
+      rewrite <- Hperm. 
+      eapply to_list_length. 
+    + intros ??;
+        eapply Hinvariants_ok; eauto. 
+      eapply Permutation_in; [symmetry|];  eassumption.
+  - shelve.
+
+    
+  - simpl. simpl.
+    eassumption.
+
+    Unshelve.
+    clear.
+    repeat match goal with
+             [H: _ |- _ ] => revert H
+           end.
+    Definition is_Some {a} (oa: option a): bool :=
+      if oa then true else false.
+
+    Definition decidesOpt {a} (op: option a) (predicate: a -> Prop):=
+      Ifopt op as s Then predicate s Else forall s, ~ predicate s.
+
+    Corollary CorrectDecoderEmptyOpt {S T}
+      : forall (monoid : Monoid T)
+          (Source_Predicate : S -> Prop)
+          (decode_inv : CacheDecode -> Prop)
+          (op : option S),
+        (Ifopt op as s Then forall s', Source_Predicate s' -> s' = s Else True) ->
+        decidesOpt op Source_Predicate 
+        -> CorrectDecoder
+            monoid
+            Source_Predicate
+            Source_Predicate
+            eq
+            empty_Format
+            (filter_decode op)
+            decode_inv
+            empty_Format.
+Proof.
+  intros.
+  destruct op.
+  - eapply ExtractViewFrom; eauto; unfold empty_Format; eauto.
+  - unfold CorrectDecoder, empty_Format; split. intros.
+    + elimtype False; eapply H0. eauto.
+    + discriminate.
+Qed.
+
+      Definition decode_filter {m} {types : Vector.t Type m} (v : list (SumType types)):
+        DecodeM ((ilist(B:=id) types) * ByteString)  ByteString:=
+        filter_decode (sortType v).
+
+
+      Definition first_check_list {m S} {types : Vector.t Type m} (v : list (SumType types))
+        ( decode2 : ilist types -> DecodeM (S * ByteString) ByteString):
+        DecodeM (S * ByteString) ByteString:=
+        sequence_Decode (decode_filter v) decode2.
+    Lemma Blah:
+      forall (S : Type) (m : nat) (types : Vector.t Type m) 
+        (projs : ilist(B:=(fun T : Type => S -> T)) types)
+        (cache_inv : CacheDecode -> Prop)
+        (view_fin : Fin.t m -> Prop) (source_pred : S -> Prop)
+        (invariants : ilist (B:=(fun T : Type => T -> Prop)) types)
+        (decode2 : ilist(B:=id) types -> DecodeM (S * ByteString) ByteString)
+        (P_inv2 : (CacheDecode -> Prop) -> Prop) (v1 : list (SumType types))
+        format2,
+        cache_inv_Property cache_inv P_inv2 ->
+        forall (Decode2_correct: forall v2 : ilist types,
+              cache_inv_Property cache_inv P_inv2 ->
+              (exists s0 : ilist types, v2 = s0 /\ sortType v1 = Some s0) ->
+              CorrectDecoder ByteStringQueueMonoid
+                (fun s : S =>
+                   (source_pred s /\ Permutation (to_list projs s) v1) /\ Some v2 = sortType v1)
+                (fun s : S =>
+                   (source_pred s /\ Permutation (to_list projs s) v1) /\ Some v2 = sortType v1)
+                eq format2 (decode2 v2) cache_inv format2) ,
+          cache_inv_Property cache_inv P_inv2 ->
+          (fun ls : list (SumType types) =>
+             (| ls |) = m /\
+               (forall x : SumType types,
+                   In x ls ->
+                   (fun st : SumType types =>
+                      view_fin (SumType_index types st) /\
+                        ith invariants (SumType_index types st) (SumType_proj types st)) x)) v1 ->
+        CorrectDecoder ByteStringQueueMonoid
+          (fun s : S => source_pred s /\ Permutation (to_list projs s) v1)
+          (fun s : S => source_pred s /\ Permutation (to_list projs s) v1) eq
+          (Compose_Format empty_Format
+             (constant (fun v2 : ilist types => Some v2 = sortType v1)) ++ 
+             format2)
+          (* (Ifopt sortType v1 as ils Then decode2 ils Else constant (constant None)) *)
+          (first_check_list v1 decode2)
+          cache_inv (Compose_Format empty_Format
+                       (constant (fun v2 : ilist types => Some v2 = sortType v1)) ++
+                       format2).
+    Proof.
+      intros.
+      unfold first_check_list.
+      eapply sequence_Compose_format_decode_correct; cycle 1.
+      - simpl; intros.
+        instantiate (1:= fun s => exists s0, s = s0 /\ sortType v1 = Some s0).
+        unshelve eapply CorrectDecoderEmptyOpt.
+        + destruct (sortType v1).
+          * simpl. intros ? [ ? []]. subst; inversion H4; reflexivity.
+          * constructor.
+        + destruct (sortType v1).
+          * simpl. eexists; split; reflexivity.
+          * simpl. intros ? [? []]. inversion H4.
+      - simpl; intros. exists v; split; eauto.
+      - simpl. eassumption. (* Hypothesis of the next format. *)
+      - unfold cache_inv_Property in *; split; eauto.
+    Qed.
+
+    intros.
+    eapply format_decode_correct_refineEquiv_Proper.
+    { instantiate (1 := (Compose_Format empty_Format
+                       (constant (fun v2 : ilist types => Some v2 = sortType v1)) ++
+                       format2)).
+      unfold flip; simpl.
+      unfold EquivFormat, refineEquiv; intros; simpl.
+Admitted.
+      
+
+Lemma Permutation_decoder'': 
+  forall (S: Type) m (types: Vector.t Type m)
+    (projs: ilist (B:= fun T => S -> T) types) (cache_inv: CacheDecode -> Prop)
+    (cache_invariants: Vector.t ((_ -> Prop) -> Prop) m) fin_cache_inv
+    (fin_format : FormatM (Fin.t m) ByteString)
+    fin_decoder view_fin
+    (fin_correct: cache_inv_Property cache_inv fin_cache_inv ->
+                        CorrectDecoder ByteStringQueueMonoid view_fin 
+                          view_fin eq fin_format fin_decoder cache_inv fin_format)
+    (formats : ilist types)
+    (source_pred : S -> Prop),
+    cache_inv_Property cache_inv
+      (fun P : CacheDecode -> Prop =>
+         fin_cache_inv P /\
+           IterateBoundedIndex.Iterate_Ensemble_BoundedIndex
+             (fun idx : Fin.t m => Vector.nth cache_invariants idx P)) ->
+    forall (invariants: ilist (B:= fun T : Type => T -> Prop) types)
+          (decoders: ilist (B:=fun T => DecodeM (T * ByteString) ByteString) types)
+          (formatrs_decoders_correct :
+            IterateBoundedIndex.Iterate_Ensemble_BoundedIndex
+              (fun idx =>
+                 cache_inv_Property cache_inv (Vector.nth cache_invariants idx)
+                 -> CorrectDecoder
+                     ByteStringQueueMonoid
+                     (ith invariants idx)
+                     (ith invariants idx)
+                     eq
+                     (ith formats idx)
+                     (ith decoders idx)
+                     cache_inv
+                     (ith formats idx)))
+        (Hinvariants_ok: forall (s : S) (v : list (SumType types)),
+            source_pred s ->
+            Permutation (to_list projs s) v ->
+            forall x : SumType types,
+              In x (to_list projs s) ->
+              view_fin (SumType_index types x) /\
+                ith invariants (SumType_index types x) (SumType_proj types x))
+        format2 (decode2: list (SumType types) -> DecodeM (S * ByteString) ByteString)
+        (P_inv2:(CacheDecode -> Prop) -> Prop)
+        (Restablish:  ilist(B:=id) types -> S)
+        (Hcache_inv2: cache_inv_Property cache_inv
+           (fun P : CacheDecode -> Prop =>
+              (fin_cache_inv P /\
+                 IterateBoundedIndex.Iterate_Ensemble_BoundedIndex'
+                   (fun idx : Fin.t m => Vector.nth cache_invariants idx P)) /\
+                P_inv2 P))
+        (Decoder2_Correct: forall v1 : list (SumType types),
+                     cache_inv_Property cache_inv P_inv2 ->
+                     (| v1 |) = m /\
+                     (forall x : SumType types,
+                      In x v1 ->
+                      view_fin (SumType_index types x) /\
+                      ith invariants (SumType_index types x) (SumType_proj types x)) ->
+                     CorrectDecoder ByteStringQueueMonoid
+                       (fun s : S => source_pred s /\ Permutation (to_list projs s) v1)
+                       (fun s : S => source_pred s /\ Permutation (to_list projs s) v1) eq format2
+                       (decode2 v1) cache_inv format2)
+        ,
+          CorrectDecoder ByteStringQueueMonoid
+                  source_pred source_pred
+                           eq 
+                           (@permutation_Format
+                              S m types projs fin_format formats
+                           )
+                           (permutation_decoder fin_decoder decoders decode2)
+                           cache_inv
+                           (@permutation_Format
+                              S m types projs fin_format formats
+                           ).
+Proof.
+  intros.
+  (* add empty*)
+  eapply format_decode_correct_refineEquiv_Proper.
+  unfold flip; simpl.
+  Lemma EquivFormat_sym {S T cach}:
+    Symmetric (@EquivFormat S T cach).
+  Admitted.
+  eapply EquivFormat_sym, sequence_mempty'.
+
+  
+  (* Real goal*)
+  unfold permutation_Format, permutation_list_Format, SumType_list_Format.
+  normalize_format. (*10.1, 10, 10*)
+  eapply sequence_Compose_format_decode_correct; cycle 1.
+  intros.
+  (* eapply strengthen_view_pred_Proper; unfold flip, pointwise_relation, impl; cycle 1. *)
+  (* eapply weaken_view_predicate_Proper; unfold flip, pointwise_relation, impl. cycle 1. *)
+  (* eapply weaken_source_pred_Proper; unfold flip, pointwise_relation, impl; simpl; cycle 1. *)
+     (* weaken_view_predicate_Proper
+      strengthen_view_pred_Proper *)
+    
+    (*1*) intros; apply FixList_decode_correct.
+  eapply IndexedSumType_Decoder_Correct; eassumption; eassumption; eassumption.
+  - simpl. intros s v Hsource Hperm.
+    split.
+    + eapply Permutation_length in Hperm.
+      rewrite <- Hperm. 
+      eapply to_list_length. 
+    + intros ??;
+        eapply Hinvariants_ok; eauto. 
+      eapply Permutation_in; [symmetry|];  eassumption.
+  - simpl. intros.
+    Ltac make_fake t:=
+      let T:= type of t in
+      let x:=fresh in evar (x:T) ; let x':= eval unfold x in x in
+                                     let HH:= fresh "HH" in
+                                     assert (HH: t=x); cycle 1; [unfold x in *; rewrite HH in *| ].
+    make_fake (decode2 v1).
+    unshelve eapply CorrectDecoderEmptyOpt.
+    + { eapply BindOpt.
+      - eapply sortType.
+        exact v1.
+      - exact (fun ils => Some (Restablish ils)). }
+    + destruct (BindOpt (sortType v1) (fun ils => Some (Restablish ils))) eqn:Heq; try solve[constructor].
+      simpl. intros ? [? ?].
+      Lemma ito_list_sortType_roundTrip:
+        forall (m : nat)
+          (types : Vector.t Type m),
+          forall x (v1: list (SumType types)),
+            Permutation (ito_list x) v1 <->
+            sortType v1 = Some x.
+      Admitted.
+      eapply ito_list_sortType_roundTrip in H4.
+      destruct (sortType v1); simpl in *; try solve [inversion Heq].
+      inversion H4; subst i.
+      assert (Restablish_Correct1: forall s, Restablish (iapp projs s) = s) by admit.
+      rewrite Restablish_Correct1 in Heq. inversion Heq; reflexivity.
+    + destruct (sortType v1) eqn:Heq.
+      * simpl.
+        unfold to_list.
+        assert (Restablish_Correct2: forall s, (iapp projs (Restablish s)) = s) by admit.
+        rewrite Restablish_Correct2.
+        split.
+        2: eapply ito_list_sortType_roundTrip; assumption.
+        admit.
+      * simpl. intros ? [].
+        eapply ito_list_sortType_roundTrip in H4.
+        rewrite H4 in Heq; inversion Heq.
+    + admit.
+  - simpl. simpl.
+    assumption.
+Qed.
+
+(* Some lemmas to modifiy themake the statment amenable to automation*)
+
+Lemma SumType_index_lift:
+  forall n (types : Vector.t Type n) (h: Type) (y : SumType types),
+    (SumType_index (Vector.cons Type h n types) (lift_SumType h y)) =
+      Fin.FS (SumType_index types y).
+Proof.
+  destruct types.
+  - intros; elim y.
+  - reflexivity.
+Qed.
+
+Lemma SumType_proj_lift:
+  forall n (types : Vector.t Type n) (h: Type) (y : SumType types),
+    let types':= (Vector.cons Type h n types) in
+    SumType_proj types y ~= SumType_proj types' (lift_SumType h y)
+.
+Proof.
+  destruct types.
+  - intros. elim y.
+  - reflexivity.
+Qed.
+
+Lemma SumType_proj_in_list:
+  forall { S : Type} {m : nat} (types : Vector.t Type m) (projs : ilist(B:= (fun T : Type => S -> T)) types) s x, 
+    In x (to_list projs s) ->
+    ith projs (SumType_index types x) s = SumType_proj types x.
+Proof.
+  induction types.
+  - intros. elim H.
+  - intros. destruct projs as [pi0 projs].
+    unfold to_list, iapp in H.
+    simpl imap in H.
+    Lemma ito_list_cons:
+      forall {n} {T:Type} {types : Vector.t Type n} (x0: T) (ils: ilist(B:=id) types),  
+        let typs := Vector.cons Type T n types in
+        ito_list (icons x0 ils) =
+          inj_SumType typs Fin.F1 x0 :: map (lift_SumType T) (@ito_list n types ils).
+    Proof. reflexivity. Qed.
+
+    rewrite ito_list_cons in H. 
+    destruct H; cycle 1.
+    + eapply in_map_iff in H.
+      destruct H as (y &Heqxy & H).
+      eapply IHtypes in H.
+      etransitivity; [rewrite <- Heqxy| reflexivity].
+      assert (LHS_lemma:
+               forall n (types : Vector.t Type n) (h: Type) (y : SumType types) S (s:S) ,
+                 let types':= (Vector.cons Type h n types) in
+                 forall (projs : ilist (B:=fun T : Type => S -> T) types'),
+                   ith projs (SumType_index types' (lift_SumType h y)) s ~=
+                     ith projs (Fin.FS (SumType_index types y)) s).
+      {
+        clear; intros.
+        subst types'.
+        erewrite SumType_index_lift.
+        econstructor.
+      }
+      eapply JMeq_eq.
+      etransitivity.
+      eapply LHS_lemma.
+      simpl.
+      rewrite H.
+
+      eapply SumType_proj_lift.
+
+    + clear IHtypes.
+      rewrite <- H.
+      destruct types; reflexivity.
+  
+
+
+Section Filter.
+
+  
+Definition filter_format {S T cache} (format: @FormatM S T cache) (condition: S -> Prop) : @FormatM S T cache:=
+fun (X : S) (X0 : CacheFormat) (X1 : T * CacheFormat) => format X X0 X1 /\ condition X.  
+
+Lemma CorrectDecoder: 
+
+
 
 Global Arguments permutation_Format {S m types} projections fin_format formats. 
 Global Opaque permutation_Format.
